fixing demo challenge 1

Dafny/control_flow.i.dfy
@@ -8,11 +8,11 @@ module control_flow {
     import opened types
     import opened memory
 
-predicate{:opaque} evalCodeOpaque(c:code, s0:state, sN:state,o:operand) 
-    { evalCode(c, s0, sN,o) }
+predicate{:opaque} evalCodeOpaque(c:code, s0:state, sN:state) 
+    { evalCode(c, s0, sN) }
 
-predicate evalCode_lax(c:code, s0:state, sN:state,o:operand) 
-    { s0.ok ==> evalCodeOpaque(c, s0, sN,o) }
+predicate evalCode_lax(c:code, s0:state, sN:state) 
+    { s0.ok ==> evalCodeOpaque(c, s0, sN) }
 
 function method lvm_CNil():codes { CNil }
 function method lvm_Block(block:codes):code { Block(block) }
@@ -37,9 +37,9 @@ function lvm_update_all(sM:lvm_state, sK:lvm_state):lvm_state{
        lvs := sM.lvs)
 }
 
-predicate {:opaque} eval_code(c:code, s:state, r:state, o:operand)
+predicate {:opaque} eval_code(c:code, s:state, r:state)
 {
-    s.ok ==> evalCode(c, s, r, o)
+    s.ok ==> evalCode(c, s, r)
 }
 
 
@@ -56,7 +56,7 @@ predicate {:opaque} eval_code(c:code, s:state, r:state, o:operand)
 
 lemma lvm_lemma_empty(s0:state, sN:state) returns(sM:state)
     // requires evalCode_lax(lvm_Block(lvm_CNil()), s0, sN, void_Operand())
-    requires exists o:operand :: eval_code(lvm_Block(lvm_CNil()), s0, sN, o)
+    requires  eval_code(lvm_Block(lvm_CNil()), s0, sN)
     ensures  s0.ok ==> sN.ok
     ensures  sM == s0
     ensures  s0.ok ==> sN == s0
@@ -66,29 +66,29 @@ lemma lvm_lemma_empty(s0:state, sN:state) returns(sM:state)
     sM := s0;
 }
 
-lemma lemma_FailurePreservedByBlock(block:codes, s:state, r:state, o:operand)
-    requires evalBlock(block, s, r, o);
+lemma lemma_FailurePreservedByBlock(block:codes, s:state, r:state)
+    requires evalBlock(block, s, r);
     ensures  !s.ok ==> !r.ok;
     decreases block;
 {
     if !block.CNil? {
-        var r' :| evalCode(block.hd, s, r', o) && evalBlock(block.tl, r', r, o);
-        lemma_FailurePreservedByCode(block.hd, s, r', o);
-        lemma_FailurePreservedByBlock(block.tl, r', r, o);
+        var r' :| evalCode(block.hd, s, r') && evalBlock(block.tl, r', r);
+        lemma_FailurePreservedByCode(block.hd, s, r');
+        lemma_FailurePreservedByBlock(block.tl, r', r);
     }
 }
 
-lemma lemma_FailurePreservedByCode(c:code, s:state, r:state, o:operand)
-    requires evalCode(c, s, r, o);
+lemma lemma_FailurePreservedByCode(c:code, s:state, r:state)
+    requires evalCode(c, s, r);
     ensures  !s.ok ==> !r.ok;
 {
     if c.Block? {
-        lemma_FailurePreservedByBlock(c.block, s, r, o);
+        lemma_FailurePreservedByBlock(c.block, s, r);
     }
 }
 
-lemma code_state_validity(c:code, s:state, r:state, o:operand)
-    requires evalCode(c, s, r, o);
+lemma code_state_validity(c:code, s:state, r:state)
+    requires evalCode(c, s, r);
     requires ValidState(s);
     decreases c, 0;
     ensures  r.ok ==> ValidState(r);
@@ -96,27 +96,27 @@ lemma code_state_validity(c:code, s:state, r:state, o:operand)
     if r.ok {
         if c.Ins? {
             assert !s.ok ==> !r.ok;
-            assert evalIns(c.ins,s,r,o);
+            assert evalIns(c.ins,s,r);
             assert s.ok;
             assert ValidInstruction(s,c.ins);
             assert r.ok;
-            assert evalIns(c.ins,s,r,o);
+            assert evalIns(c.ins,s,r);
             assert c.ins.RET? ==> ValidState(r);
 
             assert MemValid(r.m);
             assert ValidState(r);
         } else if c.Block? {
-            block_state_validity(c.block, s, r, o);
+            block_state_validity(c.block, s, r);
         } else if c.IfElse? {
                 var s' :| branchRelation(s, s', c.ifCond) &&
                     if c.ifCond then
-                        evalCode(c.ifTrue, s', r, o)
+                        evalCode(c.ifTrue, s', r)
                     else
-                        evalCode(c.ifFalse, s', r, o);
+                        evalCode(c.ifFalse, s', r);
                 if c.ifCond {
-                    code_state_validity(c.ifTrue, s', r, o);
+                    code_state_validity(c.ifTrue, s', r);
                 } else {
-                    code_state_validity(c.ifFalse, s', r, o);
+                    code_state_validity(c.ifFalse, s', r);
                 }
             assert ValidState(r);
         } 
@@ -128,32 +128,32 @@ lemma code_state_validity(c:code, s:state, r:state, o:operand)
     }
 }
 
-lemma block_state_validity(block:codes, s:state, r:state, o:operand)
-    requires evalBlock(block, s, r, o);
+lemma block_state_validity(block:codes, s:state, r:state)
+    requires evalBlock(block, s, r);
     requires ValidState(s);
     decreases block, 0;
     ensures  r.ok ==> ValidState(r);
 {
     if block.lvm_CCons? {
-        var r':state :| evalCode(block.hd, s, r', o) && evalBlock(block.tl, r', r, o);
-        code_state_validity(block.hd, s, r', o);
+        var r':state :| evalCode(block.hd, s, r') && evalBlock(block.tl, r', r);
+        code_state_validity(block.hd, s, r');
         if r'.ok {
-            block_state_validity(block.tl, r', r, o);
+            block_state_validity(block.tl, r', r);
         }
         else {
-            lemma_FailurePreservedByBlock(block.tl, r', r, o);
+            lemma_FailurePreservedByBlock(block.tl, r', r);
         }
     }
 }
 
 
-lemma lvm_lemma_block_lax(b0:lvm_codes, s0:state, sN:state,o:operand) 
+lemma lvm_lemma_block_lax(b0:lvm_codes, s0:state, sN:state) 
                 returns(s1:state, c1:lvm_code, b1:lvm_codes)
     requires b0.lvm_CCons?
-    requires evalCode_lax(lvm_Block(b0), s0, sN,o)
+    requires evalCode_lax(lvm_Block(b0), s0, sN)
     ensures  b0 == lvm_CCons(c1, b1)
-    ensures  evalCode_lax(c1, s0, s1,o)
-    ensures  evalCode_lax(lvm_Block(b1), s1, sN,o)
+    ensures  evalCode_lax(c1, s0, s1)
+    ensures  evalCode_lax(lvm_Block(b1), s1, sN)
     // ensures StateNext(s0,s1)
 {
     reveal_evalCodeOpaque();
@@ -161,13 +161,13 @@ lemma lvm_lemma_block_lax(b0:lvm_codes, s0:state, sN:state,o:operand)
     b1 := b0.tl;
     if (s0.ok)
     {
-        assert evalBlock(b0, s0, sN,o);
-        var r':state :| evalCode(b0.hd, s0, r',o) && evalBlock(b0.tl, r', sN,o);
+        assert evalBlock(b0, s0, sN);
+        var r':state :| evalCode(b0.hd, s0, r') && evalBlock(b0.tl, r', sN);
         s1 := r';
         if ValidState(s0) {
-            code_state_validity(c1, s0, s1,o);
+            code_state_validity(c1, s0, s1);
         }
-        assert evalCode_lax(c1, s0, s1,o);
+        assert evalCode_lax(c1, s0, s1);
         // s1 :| evalCode(b0.hd, s0, s1,o) && (if s1.ok then evalBlock(b0.tl, s1, sN,o) else s1 == sN);
     }
     else
@@ -176,50 +176,50 @@ lemma lvm_lemma_block_lax(b0:lvm_codes, s0:state, sN:state,o:operand)
     }
 }
 
-lemma lvm_lemma_block(b:codes, s0:lvm_state, r:lvm_state,o:operand) 
+lemma lvm_lemma_block(b:codes, s0:lvm_state, r:lvm_state) 
                 returns(r1:lvm_state, c0:code, b1:codes)
     requires b.lvm_CCons?
-    requires eval_code(Block(b), s0, r,o)
+    requires eval_code(Block(b), s0, r)
     ensures  b == lvm_CCons(c0, b1)
     ensures  ValidState(s0) && r1.ok ==> ValidState(r1);
-    ensures  eval_code(c0, s0, r1,o)
-    ensures  eval_code(Block(b1), r1, r,o)
-    ensures s0.ok ==> evalCode(b.hd, s0, r1,o) && evalBlock(b.tl, r1, r,o);
+    ensures  eval_code(c0, s0, r1)
+    ensures  eval_code(Block(b1), r1, r)
+    ensures s0.ok ==> evalCode(b.hd, s0, r1) && evalBlock(b.tl, r1, r);
     ensures s0.ok && b.hd.Block? ==> r1 == s0;
 {
     reveal_eval_code();
     c0 := b.hd;
     b1 := b.tl;
     if s0.ok {
-        assert evalBlock(b, s0, r,o);
-        var r':state :| evalCode(b.hd, s0, r',o) && evalBlock(b.tl, r', r,o)  && (b.hd.Block? ==> s0 == r');
+        assert evalBlock(b, s0, r);
+        var r':state :| evalCode(b.hd, s0, r') && evalBlock(b.tl, r', r)  && (b.hd.Block? ==> s0 == r');
         r1 := r';
         if ValidState(s0) {
-            code_state_validity(c0, s0, r1,o);
+            code_state_validity(c0, s0, r1);
         }
         if(b.hd.Block?){
             assert r1 == s0;
         }
-        assert eval_code(c0, s0, r1,o);
+        assert eval_code(c0, s0, r1);
     } else {
         r1 := s0;
     }
 }
 
-predicate lvm_require(block0:lvm_codes, c:lvm_code, s0:lvm_state, sN:lvm_state,o:operand)
+predicate lvm_require(block0:lvm_codes, c:lvm_code, s0:lvm_state, sN:lvm_state)
 {
     block0.lvm_CCons?
  && block0.hd == c
- && evalCode_lax(lvm_Block(block0), s0, sN,o)
+ && evalCode_lax(lvm_Block(block0), s0, sN)
  && ValidState(s0)
 }
 
-predicate lvm_ensure(b0:lvm_codes, b1:lvm_codes, s0:lvm_state, s1:lvm_state, sN:lvm_state,o:operand)
+predicate lvm_ensure(b0:lvm_codes, b1:lvm_codes, s0:lvm_state, s1:lvm_state, sN:lvm_state)
 {
     b0.lvm_CCons?
  && b0.tl == b1
- && (s1.ok ==> evalCode_lax(b0.hd, s0, s1,o))
- && evalCode_lax(lvm_Block(b1), s1, sN,o)
+ && (s1.ok ==> evalCode_lax(b0.hd, s0, s1))
+ && evalCode_lax(lvm_Block(b1), s1, sN)
  && ValidState(s1)
 }
 
@@ -230,6 +230,7 @@ type lvm_codes = codes
 type lvm_state = state
 type lvm_operand_opr = operand
 type lvm_data = Data
+type lvm_cond = condition
 
 function lvm_get_ok(s:lvm_state):bool { ValidState(s) }
 predicate lvm_is_src_opr(o:operand, s:lvm_state) { true }
