Dafny/llvm.i.dfy
@@ -5,12 +5,14 @@ include "./Operations/conversionOperations.i.dfy"
 include "./Operations/bitwiseBinaryOperations.i.dfy"
 include "./Operations/binaryOperations.i.dfy"
 include "./Operations/otherOperations.i.dfy"
+include "./Libraries/SeqIsUniqueDef.i.dfy"
 
 module LLVM_def {
 
     import opened types
     import opened ops
     import opened memory
+    import opened Common__SeqIsUniqueDef_i
     import opened conversion_operations_i
     import opened bitwise_binary_operations_i
     import opened binary_operations_i
@@ -117,7 +119,7 @@ module LLVM_def {
     {
         ValidState(s)
         && ValidState(s')
-        && exists ins,o :: (ValidInstruction(s,ins) && evalIns(ins, s, s',o))
+        && exists ins :: (ValidInstruction(s,ins) && evalIns(ins, s, s'))
     }
 
     predicate ValidOperand(s:state,o:operand)
@@ -228,6 +230,8 @@ module LLVM_def {
         ensures evalUpdate(s, o, data, r) ==> ValidData(r,data)
         ensures evalUpdate(s, o, data, r) ==> ValidRegOperand(r,o)
         ensures evalUpdate(s, o, data, r) ==> ValidOperand(r,o)
+        ensures evalUpdate(s, o, data, r) ==> 
+        (forall d :: ValidOperand(s,d) && d != o ==> ValidOperand(r,d) && OperandContents(s,d) == OperandContents(r,d));
 
     {
         reveal_ValidRegState();
@@ -271,54 +275,56 @@ module LLVM_def {
 
     // lemma equalStatesEqualOperands(s:state, s':state, o:operand)
     //     requires ValidState(s)
-    predicate evalIns(ins:ins, s:state, r:state,o:operand)
+    predicate evalIns(ins:ins, s:state, r:state)
     {   
         if !s.ok || !ValidInstruction(s, ins) then !r.ok
         else match ins
-            case ADD(dst,t,src1,src2) => o == dst 
+            case ADD(dst,t,src1,src2) => //o == dst 
                                 && ValidData(r,evalADD(t,OperandContents(s,src1),OperandContents(s,src2))) 
                                 && evalUpdate(s, dst, evalADD(t,OperandContents(s,src1),OperandContents(s,src2)),r)
-            case SUB(dst,t,src1,src2) => o == dst 
+            case SUB(dst,t,src1,src2) => //o == dst 
                                 && ValidData(r,evalSUB(t,OperandContents(s,src1),OperandContents(s,src2))) 
                                 && evalUpdate(s, dst, evalSUB(t,OperandContents(s,src1),OperandContents(s,src2)),r)
-            case CALL(dst,fnc) => o == dst 
-                                && evalCode(fnc,s,r,o) 
-                                && ValidData(r,OperandContents(s,o))
-                                && evalUpdate(s,dst,OperandContents(s,o),r)
-            case GETELEMENTPTR(dst,t,op1,op2) => o == dst 
+            case CALL(dst,fnc) => //o == dst 
+                                && evalCode(fnc,s,r) 
+                                && ValidData(r,OperandContents(s,dst))
+                                && evalUpdate(s,dst,OperandContents(s,dst),r)
+            case GETELEMENTPTR(dst,t,op1,op2) => //o == dst 
                                 && ValidData(r,evalGETELEMENTPTR(s.m,t,OperandContents(s,op1),OperandContents(s,op2)))
                                 && evalUpdate(s, dst, evalGETELEMENTPTR(s.m,t,OperandContents(s,op1),OperandContents(s,op2)),r)
-            case ICMP(dst,cond,t,src1,src2) => o == dst 
+            case ICMP(dst,cond,t,src1,src2) => //o == dst 
                                 && ValidData(r,evalICMP(cond,t,OperandContents(s,src1),OperandContents(s,src2)))
                                 && evalUpdate(s, dst, evalICMP(cond,t,OperandContents(s,src1),OperandContents(s,src2)),r)
+                                && OperandContents(s,src1).itype == OperandContents(r,src1).itype
             case RET(val) => ValidState(r) && 
                     if OperandContents(s,val).Void? then r == s
-                    else o == val  && evalUpdate(s, o, OperandContents(s,val),r)// && r == s
+                    else //o == val  
+                    && evalUpdate(s, val, OperandContents(s,val),r)// && r == s
             // case RET(dst, val) => && ValidData(r,OperandContents(s,val)) 
             //                       && if OperandContents(s,val).Void? then s == r else evalUpdate(s, dst, OperandContents(s,val),r)//evalRet(s,dst,OperandContents(s,val),r)// o == val && ValidState(r) //&& r == s
-            case BR(cond, labelTrue,labelFalse) => evalIfElse(cond,labelTrue,labelFalse,s,r,o)&& ValidState(r)
-            case SHL(dst,src,shiftAmt) =>o == dst
+            case BR(cond, labelTrue,labelFalse) => evalIfElse(cond,labelTrue,labelFalse,s,r)&& ValidState(r)
+            case SHL(dst,src,shiftAmt) =>//o == dst
                                 && ValidData(r,evalSHL(OperandContents(s,src),OperandContents(s,shiftAmt)))
                                 && evalUpdate(s, dst, evalSHL(OperandContents(s,src),OperandContents(s,shiftAmt)),r)
-            case LSHR(dst,src,shiftAmt) => o == dst 
+            case LSHR(dst,src,shiftAmt) =>// o == dst 
                                 && ValidData(r,evalLSHR(OperandContents(s,src),OperandContents(s,shiftAmt)))
                                 && evalUpdate(s, dst, evalLSHR(OperandContents(s,src),OperandContents(s,shiftAmt)),r)
-            case AND(dst,src1,src2) => o == dst 
+            case AND(dst,src1,src2) => //o == dst 
                                 && ValidData(r,evalAND(OperandContents(s,dst).itype.size,OperandContents(s,src1),OperandContents(s,src2)))   
                                 && evalUpdate(s, dst, evalAND(OperandContents(s,dst).itype.size,OperandContents(s,src1),OperandContents(s,src2)),r)
-            case OR(dst,src1,src2) => o == dst 
+            case OR(dst,src1,src2) => //o == dst 
                                 && ValidData(r,evalOR(OperandContents(s,dst).itype.size,OperandContents(s,src1),OperandContents(s,src2)))   
                                 && evalUpdate(s, dst, evalOR(OperandContents(s,dst).itype.size,OperandContents(s,src1),OperandContents(s,src2)),r)
-            case TRUN(dst,t,src,dstSize) => o == dst
+            case TRUN(dst,t,src,dstSize) => //o == dst
                                 && ValidData(r,evalTRUNC(OperandContents(s,src),dstSize))    
                                 && evalUpdate(s, dst, evalTRUNC(OperandContents(s,src),dstSize),r)
-            case SEXT(dst,t,src,dstSize) => o == dst
+            case SEXT(dst,t,src,dstSize) => //o == dst
                                 && ValidData(r,evalSEXT(OperandContents(s,src),dstSize))    
                                 && evalUpdate(s, dst, evalSEXT(OperandContents(s,src),dstSize),r)
-            case ZEXT(dst,t,src,dstSize) => o == dst 
+            case ZEXT(dst,t,src,dstSize) =>// o == dst 
                                 && ValidData(r,evalZEXT(OperandContents(s,src),dstSize))
                                 && evalUpdate(s, dst, evalZEXT(OperandContents(s,src),dstSize),r)
-            case LOAD(dst,mems,size,src) => o == dst 
+            case LOAD(dst,mems,size,src) =>// o == dst 
                                 && s.m == r.m
                                 // && exists d:Data :: Load(s.m,r.m,OperandContents(s,src).bid,OperandContents(s,src).offset,d) 
                                 && evalUpdate(s, dst, evalLOAD(s.m,r.m,size,OperandContents(s,src)),r)
@@ -329,12 +335,12 @@ module LLVM_def {
             case EXTRACTVALUE() => ValidState(r)   
     }
 
-    predicate evalBlock(block:codes, s:state, r:state, o:operand)
+    predicate evalBlock(block:codes, s:state, r:state)
     {
         if block.CNil? then
             r == s
         else
-            exists r' :: (evalCode(block.hd, s, r',o) && evalBlock(block.tl, r', r,o)
+            exists r' :: (evalCode(block.hd, s, r') && evalBlock(block.tl, r', r)
             && (block.hd.Block? ==> s == r'))
     }
 
@@ -352,22 +358,56 @@ module LLVM_def {
         dataToBool(evalICMP(o.cmp, OperandContents(s, o.o1).itype.size, OperandContents(s, o.o1), OperandContents(s, o.o2)))
     }
 
-    predicate evalIfElse(cond:bool, ifT:code, ifF:code, s:state, r:state,o:operand)
+    predicate evalIfElse(cond:bool, ifT:code, ifF:code, s:state, r:state)
         decreases if ValidState(s) && cond then ifT else ifF
     {
         if ValidState(s) && s.ok then
-            exists s' :: branchRelation(s, s', cond) && (if cond then evalCode(ifT, s', r,o) else evalCode(ifF, s', r,o))
+            exists s' :: branchRelation(s, s', cond) && (if cond then evalCode(ifT, s', r) else evalCode(ifF, s', r))
         else
             !r.ok
     }
 
-    predicate evalCode(c:code, s:state, r:state, o:operand)
+    predicate evalCode(c:code, s:state, r:state)
         decreases c, 0
     {
         match c
-            case Ins(ins) => evalIns(ins, s, r, o)
-            case Block(block) => evalBlock(block, s, r,o)
-            case IfElse(cond, ifT, ifF) => evalIfElse(cond, ifT, ifF, s, r,o)
+            case Ins(ins) => evalIns(ins, s, r)
+            case Block(block) => evalBlock(block, s, r)
+            case IfElse(cond, ifT, ifF) => evalIfElse(cond, ifT, ifF, s, r)
     }
+
+//// utility functions
+
+    function copyIntOperand(s:Data) : (out:operand)
+        requires s.Int?
+        ensures out.D? && out.d.Int?
+        ensures out.d.val == s.val 
+        ensures out.d.itype.size == s.itype.size
+        ensures out.d.itype.signed == s.itype.signed;
+    {
+        var x:operand := D(Int(s.val,IntType(s.itype.size,s.itype.signed)));
+        x
+    }
+
+    function copyPtrOperand(s:Data) : (out:operand)
+        requires s.Ptr?
+        ensures out.D? && out.d.Ptr?
+        ensures out.d.block == s.block 
+        ensures out.d.bid == s.bid
+        ensures out.d.offset == s.offset;
+    {
+        var x:operand := D(Ptr(s.block, s.bid, s.offset));
+        x
+    }
+
+    predicate operandsUnique(s:state,ops:seq<operand>)
+        requires ValidState(s)
+        requires forall o :: o in ops ==> ValidOperand(s,o)
+    {
+        reveal_SeqIsUnique();
+        reveal_SeqIsUniqueAtomic();
+        SeqIsUnique(ops) && SeqIsUniqueAtomic(ops)
+    }
+
 
 }
