Dafny/examples/generalInstructions.i.dfy
@@ -5,6 +5,7 @@ include "../memory.dfy"
 include "../Operations/binaryOperations.i.dfy"
 include "../Operations/conversionOperations.i.dfy"
 include "../Operations/bitwiseBinaryOperations.i.dfy"
+include "../Operations/otherOperations.i.dfy"
 
 module general_instructions {
     import opened LLVM_def
@@ -14,6 +15,7 @@ module general_instructions {
     import opened binary_operations_i
     import opened conversion_operations_i
     import opened bitwise_binary_operations_i
+    import opened other_operations_i
 
 function method{:opaque}lvm_code_Add(dst:lvm_operand_opr, size:nat, src1:lvm_operand_opr,src2:lvm_operand_opr):lvm_code
 
@@ -21,10 +23,10 @@ function method{:opaque}lvm_code_Add(dst:lvm_operand_opr, size:nat, src1:lvm_ope
    Ins(ADD(dst, size,src1,src2))
 }
 lemma lvm_lemma_Add(lvm_b0:lvm_codes, lvm_s0:lvm_state, lvm_sN:lvm_state, 
-            dst:lvm_operand_opr, size:nat, src1:lvm_operand_opr,src2:lvm_operand_opr,o:operand)
+            dst:lvm_operand_opr, size:nat, src1:lvm_operand_opr,src2:lvm_operand_opr)
   returns (lvm_bM:lvm_codes, lvm_sM:lvm_state)
 
-  requires lvm_require(lvm_b0, lvm_code_Add(dst, size,src1,src2), lvm_s0, lvm_sN,dst)
+  requires lvm_require(lvm_b0, lvm_code_Add(dst, size,src1,src2), lvm_s0, lvm_sN)
   requires lvm_is_dst_opr(dst, lvm_s0)
   requires lvm_is_src_opr(src1, lvm_s0)
   requires lvm_get_ok(lvm_s0)
@@ -42,7 +44,7 @@ lemma lvm_lemma_Add(lvm_b0:lvm_codes, lvm_s0:lvm_state, lvm_sN:lvm_state,
   requires lvm_code_Add(dst, size,src1,src2).Ins?;
   requires ValidOperand(lvm_s0,dst)
 // //   
-  ensures  lvm_ensure(lvm_b0, lvm_bM, lvm_s0, lvm_sM, lvm_sN,dst)
+  ensures  lvm_ensure(lvm_b0, lvm_bM, lvm_s0, lvm_sM, lvm_sN)
   ensures  lvm_get_ok(lvm_sM)
   ensures  ValidOperand(lvm_sM,dst)
   ensures  ValidOperand(lvm_sM,src1)
@@ -54,11 +56,11 @@ lemma lvm_lemma_Add(lvm_b0:lvm_codes, lvm_s0:lvm_state, lvm_sN:lvm_state,
   ensures  OperandContents(lvm_sM,dst).Int?;
   ensures  lvm_state_eq(lvm_sM, lvm_update_mem( lvm_sM, lvm_update_all(lvm_sM, lvm_s0)))
   ensures  lvm_state_eq(lvm_sM, lvm_update_ok(lvm_sM, lvm_update_all( lvm_sM, lvm_s0)))
-  ensures  forall s2 :: evalCode(lvm_b0.hd, lvm_s0, s2,o) ==> s2.ok
+  ensures  forall s2 :: evalCode(lvm_b0.hd, lvm_s0, s2) ==> s2.ok
   ensures OperandContents(lvm_sM, dst).val == evalADD(OperandContents(lvm_s0,dst).itype.size,OperandContents(lvm_s0,src1),OperandContents(lvm_s0,src2)).val;
   ensures ToTwosComp(OperandContents(lvm_sM, dst)).val == 
           (OperandContents(lvm_s0, src1).val + OperandContents(lvm_s0, src2).val) % Pow256(OperandContents(lvm_s0, src1).itype.size)
-
+  ensures forall d :: ValidOperand(lvm_s0,d) && d != dst ==> ValidOperand(lvm_sM,d) && OperandContents(lvm_s0,d) == OperandContents(lvm_sM,d)
 {
     reveal_lvm_code_Add();
     reveal_evalCodeOpaque();
@@ -70,13 +72,13 @@ lemma lvm_lemma_Add(lvm_b0:lvm_codes, lvm_s0:lvm_state, lvm_sN:lvm_state,
     assert  ValidRegOperand(lvm_s0, dst);
     assert ValidState(lvm_s0);
     var lvm_old_s:lvm_state := lvm_s0;
-    assert evalCode_lax(lvm_Block(lvm_b0), lvm_s0, lvm_sN,dst);
+    assert evalCode_lax(lvm_Block(lvm_b0), lvm_s0, lvm_sN);
     assert lvm_s0.ok;
-    assert eval_code(lvm_Block(lvm_b0), lvm_s0, lvm_sN,dst);
-    assert evalBlock(lvm_Block(lvm_b0).block, lvm_s0, lvm_sN,dst);
-    assert exists r' :: (evalCode(lvm_b0.hd, lvm_s0, r',dst));
+    assert eval_code(lvm_Block(lvm_b0), lvm_s0, lvm_sN);
+    assert evalBlock(lvm_Block(lvm_b0).block, lvm_s0, lvm_sN);
+    assert exists r' :: (evalCode(lvm_b0.hd, lvm_s0, r'));
 
-    ghost var lvm_ltmp1, lvm_cM:lvm_code, lvm_ltmp2 := lvm_lemma_block(lvm_b0, lvm_s0, lvm_sN,dst);
+    ghost var lvm_ltmp1, lvm_cM:lvm_code, lvm_ltmp2 := lvm_lemma_block(lvm_b0, lvm_s0, lvm_sN);
     lvm_sM := lvm_ltmp1;
     lvm_bM := lvm_ltmp2;
     assert lvm_b0.tl == lvm_bM;
@@ -84,8 +86,10 @@ lemma lvm_lemma_Add(lvm_b0:lvm_codes, lvm_s0:lvm_state, lvm_sN:lvm_state,
     assert lvm_s0.ok;
     assert ValidState(lvm_sM);
     assert ValidOperand(lvm_sM,dst);
-    assert evalIns(lvm_code_Add(dst, size,src1,src2).ins,lvm_s0,lvm_sM,dst);
-    assert evalUpdate(lvm_s0, dst, evalADD(OperandContents(lvm_s0,dst).itype.size,OperandContents(lvm_s0,src1),OperandContents(lvm_s0,src2)),lvm_sM);
+    assert evalIns(lvm_code_Add(dst, size,src1,src2).ins,lvm_s0,lvm_sM);
+    var evalA := evalADD(OperandContents(lvm_s0,dst).itype.size,OperandContents(lvm_s0,src1),OperandContents(lvm_s0,src2));
+    assert evalUpdate(lvm_s0, dst, evalA,lvm_sM);
+    assert (forall d :: ValidOperand(lvm_s0,d) && d != dst ==> ValidOperand(lvm_sM,d) && OperandContents(lvm_s0,d) == OperandContents(lvm_sM,d));
     assert ValidData(lvm_sM,evalADD(OperandContents(lvm_s0,dst).itype.size,OperandContents(lvm_s0,src1),OperandContents(lvm_s0,src2)));
     assert OperandContents(lvm_sM, dst).val == evalADD(OperandContents(lvm_s0,dst).itype.size,OperandContents(lvm_s0,src1),OperandContents(lvm_s0,src2)).val;
     reveal_evalCodeOpaque();
@@ -103,7 +107,7 @@ lemma lvm_lemma_GetElementPtr(lvm_b0:lvm_codes, lvm_s0:lvm_state, lvm_sN:lvm_sta
             dst:lvm_operand_opr,s:MemState,t:bitWidth,op1:lvm_operand_opr,op2:lvm_operand_opr)
   returns (lvm_bM:lvm_codes, lvm_sM:lvm_state)
   
-  requires lvm_require(lvm_b0, lvm_code_GetElementPtr(dst,t,op1,op2), lvm_s0, lvm_sN,dst)
+  requires lvm_require(lvm_b0, lvm_code_GetElementPtr(dst,t,op1,op2), lvm_s0, lvm_sN)
   requires lvm_is_dst_opr(dst, lvm_s0)
   requires lvm_is_src_opr(op1, lvm_s0)
   requires lvm_get_ok(lvm_s0)
@@ -118,22 +122,24 @@ lemma lvm_lemma_GetElementPtr(lvm_b0:lvm_codes, lvm_s0:lvm_state, lvm_sN:lvm_sta
   requires ValidOperand(lvm_s0,dst)
 //   
 ensures lvm_s0.m == lvm_sM.m;
-  ensures  lvm_ensure(lvm_b0, lvm_bM, lvm_s0, lvm_sM, lvm_sN,dst)
+  ensures  lvm_ensure(lvm_b0, lvm_bM, lvm_s0, lvm_sM, lvm_sN)
   ensures  lvm_get_ok(lvm_sM)
   ensures ValidOperand(lvm_sM,dst)
 
   ensures OperandContents(lvm_sM,dst).Ptr?;
   ensures  OperandContents(lvm_sM, dst) == evalGETELEMENTPTR(lvm_s0.m,t,OperandContents(lvm_s0,op1),OperandContents(lvm_s0,op2));
   ensures  lvm_state_eq(lvm_sM, lvm_update_ok(lvm_sM, lvm_update_all( lvm_sM, lvm_s0)))
+  ensures forall d :: ValidOperand(lvm_s0,d) && d != dst ==> ValidOperand(lvm_sM,d) && OperandContents(lvm_s0,d) == OperandContents(lvm_sM,d)
+
 {
   reveal_lvm_code_GetElementPtr();
   reveal_ValidData();
   reveal_evalCodeOpaque();
   reveal_eval_code();
 
-  assert evalBlock(lvm_b0, lvm_s0, lvm_sN,dst);
+  assert evalBlock(lvm_b0, lvm_s0, lvm_sN);
 
-  ghost var lvm_ltmp1, lvm_cM:lvm_code, lvm_ltmp2 := lvm_lemma_block(lvm_b0, lvm_s0, lvm_sN,dst);
+  ghost var lvm_ltmp1, lvm_cM:lvm_code, lvm_ltmp2 := lvm_lemma_block(lvm_b0, lvm_s0, lvm_sN);
   lvm_sM := lvm_ltmp1;
   lvm_bM := lvm_ltmp2;
 //   var lvm_b1:lvm_codes := lvm_get_block(lvm_cM);
@@ -141,12 +147,12 @@ ensures lvm_s0.m == lvm_sM.m;
       assert lvm_b0.tl == lvm_bM;
 
   assert ValidState(lvm_sM);
-  assert evalCode_lax(lvm_cM, lvm_s0, lvm_sM,dst);
+  assert evalCode_lax(lvm_cM, lvm_s0, lvm_sM);
   reveal_evalCodeOpaque();
 }
 
 
-function method{:opaque} lvm_RET(op1:lvm_operand_opr):lvm_code
+function method{:opaque} lvm_code_Ret(op1:lvm_operand_opr):lvm_code
 {
     //getelementptr
     reveal_IntFits();
@@ -157,7 +163,7 @@ function method{:opaque} lvm_RET(op1:lvm_operand_opr):lvm_code
 lemma lvm_lemma_Ret(lvm_b0:lvm_codes, lvm_s0:lvm_state, lvm_sN:lvm_state,dst:lvm_operand_opr, op1:lvm_operand_opr)
   returns (lvm_bM:lvm_codes, lvm_sM:lvm_state)
   
-  requires lvm_require(lvm_b0, lvm_RET(op1), lvm_s0, lvm_sN,dst)
+  requires lvm_require(lvm_b0, lvm_code_Ret(op1), lvm_s0, lvm_sN)
   requires lvm_is_dst_opr(dst, lvm_s0)
   requires lvm_is_src_opr(op1, lvm_s0)
   requires lvm_get_ok(lvm_s0)
@@ -165,20 +171,22 @@ lemma lvm_lemma_Ret(lvm_b0:lvm_codes, lvm_s0:lvm_state, lvm_sN:lvm_state,dst:lvm
   requires ValidOperand(lvm_s0,op1);
 
 //   
-  ensures  lvm_ensure(lvm_b0, lvm_bM, lvm_s0, lvm_sM, lvm_sN,dst)
+  ensures  lvm_ensure(lvm_b0, lvm_bM, lvm_s0, lvm_sM, lvm_sN)
   ensures  lvm_get_ok(lvm_sM)
   ensures  OperandContents(lvm_s0,op1).Void? ==> lvm_s0 == lvm_sM
   ensures  lvm_state_eq(lvm_sM,  lvm_s0)
   ensures lvm_bM == lvm_b0.tl;
+    ensures forall d :: ValidOperand(lvm_s0,d) && d != dst ==> ValidOperand(lvm_sM,d) && OperandContents(lvm_s0,d) == OperandContents(lvm_sM,d)
+
 {
-  reveal_lvm_RET();
+  reveal_lvm_code_Ret();
   reveal_ValidData();
   reveal_evalCodeOpaque();
   reveal_eval_code();
 
-  assert evalBlock(lvm_b0, lvm_s0, lvm_sN,dst);
+  assert evalBlock(lvm_b0, lvm_s0, lvm_sN);
 
-  ghost var lvm_ltmp1, lvm_cM:lvm_code, lvm_ltmp2 := lvm_lemma_block(lvm_b0, lvm_s0, lvm_sN,dst);
+  ghost var lvm_ltmp1, lvm_cM:lvm_code, lvm_ltmp2 := lvm_lemma_block(lvm_b0, lvm_s0, lvm_sN);
   lvm_sM := lvm_ltmp1;
   lvm_bM := lvm_ltmp2;
 //   var lvm_b1:lvm_codes := lvm_get_block(lvm_cM);
@@ -186,109 +194,10 @@ lemma lvm_lemma_Ret(lvm_b0:lvm_codes, lvm_s0:lvm_state, lvm_sN:lvm_state,dst:lvm
   assert lvm_b0.tl == lvm_bM;
 
   assert ValidState(lvm_sM);
-  assert evalCode(lvm_cM, lvm_s0, lvm_sM,dst);
+  assert evalCode(lvm_cM, lvm_s0, lvm_sM);
   reveal_evalCodeOpaque();
 }
 
-// lemma lvm_lemma_Ret(lvm_b0:lvm_codes, lvm_s0:lvm_state, lvm_sN:lvm_state,dst:lvm_operand_opr,op1:lvm_operand_opr)
-//   returns (lvm_bM:lvm_codes, lvm_sM:lvm_state)
-  
-//   requires exists a :: lvm_require(lvm_b0, lvm_RET(dst,op1), lvm_s0, lvm_sN,a)
-//   requires lvm_is_dst_opr(dst, lvm_s0)
-//   requires lvm_is_src_opr(op1, lvm_s0)
-//   requires lvm_get_ok(lvm_s0)
-//   requires ValidOperand(lvm_s0,dst);
-
-//   requires ValidOperand(lvm_s0,op1);
-
-// //   
-//   ensures  lvm_ensure(lvm_b0, lvm_bM, lvm_s0, lvm_sM, lvm_sN,dst)
-//   ensures  lvm_get_ok(lvm_sM)
-//   // ensures lvm_s0 == lvm_sM
-//   // ensures  lvm_state_eq(lvm_sM,  lvm_s0)
-// {
-//   reveal_lvm_RET();
-//   reveal_ValidData();
-//   reveal_evalCodeOpaque();
-//   reveal_eval_code();
-
-//   assert lvm_b0.hd.Ins? && lvm_b0.hd.ins.RET?;
-//   // dst :| evalBlock(lvm_b0, lvm_s0, lvm_sN,dst);
-//   // assert evalBlock(lvm_b0, lvm_s0, lvm_sN,dst);
-//       // assert eval_code(lvm_Block(lvm_b0), lvm_s0, lvm_sN,dst);
-
-//   // assert ValidInstruction(lvm_s0, lvm_b0.hd.ins);
-//   // assert exists r' :: ValidData(r',OperandContents(lvm_s0,lvm_b0.hd.ins.val));
-//   // assert exists r' :: (evalCode(lvm_b0.hd, lvm_s0, r',dst)); //&& evalBlock(lvm_b0.tl, r', lvm_sN,dst));
-//   // assert if lvm_b0.hd.ins.val.Void? then evalRet(lvm_s0, dst, lvm_b0.hd.ins.val, lvm_s0) 
-//   // else evalUpdate(lvm_s0, dst, lvm_b0.hd.ins.val, lvm_s0);
-//     // && OperandContents(lvm_s0, dst) == OperandContents(r', dst));
-          
-//   // assert exists r' :: (evalIns(lvm_b0.hd.ins, lvm_s0, r',dst));
-
-//   // assert evalBlock(lvm_b0, lvm_s0, lvm_sN,dst);
-
-//   // var r :| (evalIns(lvm_b0.hd.ins, lvm_s0, r,dst));
-//   // assert eval_code(Block(lvm_b0), lvm_s0, lvm_sN,dst);
-
-//   // assert dst == op1;
-
-//   ghost var lvm_ltmp1, lvm_cM:lvm_code, lvm_ltmp2 := lvm_lemma_block(lvm_b0, lvm_s0, lvm_sN,dst);
-//   lvm_sM := lvm_ltmp1;
-//   lvm_bM := lvm_ltmp2;
-// //   var lvm_b1:lvm_codes := lvm_get_block(lvm_cM);
-//   assert lvm_sM.ok;
-//   assert lvm_b0.tl == lvm_bM;
-
-//   assert ValidState(lvm_sM);
-//   assert evalCode_lax(lvm_cM, lvm_s0, lvm_sM,dst);
-//   reveal_evalCodeOpaque();
-// }
-
-
-
-// lemma lvm_lemma_Ret(lvm_b0:lvm_codes, lvm_s0:lvm_state, lvm_sN:lvm_state, op1:lvm_operand_opr)
-//   returns (lvm_bM:lvm_codes, lvm_sM:lvm_state, lvm_ret:lvm_operand_opr)
-  
-//   requires lvm_require(lvm_b0, lvm_RET(op1), lvm_s0, lvm_sN,op1)
-//   // requires lvm_is_dst_opr(lvm_ret, lvm_s0)
-//   requires lvm_is_src_opr(op1, lvm_s0)
-//   requires lvm_get_ok(lvm_s0)
-
-//   requires ValidOperand(lvm_s0,op1);
-
-// //   
-//   ensures  lvm_ensure(lvm_b0, lvm_bM, lvm_s0, lvm_sM, lvm_sN,lvm_ret)
-//   ensures  lvm_get_ok(lvm_sM)
-//   // ensures  lvm_s0 == lvm_sM
-//   // ensures ValidOperand(lvm_sM,op1);
-//   // ensures ValidOperand(lvm_sM,lvm_ret);
-//   // ensures OperandContents(lvm_sM,op1) ==  OperandContents(lvm_sM,lvm_ret);
-//   // ensures  lvm_state_eq(lvm_sM,  lvm_s0)
-// {
-//   reveal_lvm_RET();
-//   reveal_ValidData();
-//   reveal_evalCodeOpaque();
-//   reveal_eval_code();
-  
-//   lvm_ret :| lvm_require(lvm_b0, lvm_RET(op1), lvm_s0, lvm_sN,lvm_ret);
-//   assert evalBlock(lvm_b0, lvm_s0, lvm_sN,lvm_ret);
-//   assert ValidInstruction(lvm_s0, lvm_RET(op1).ins);
-
-//   ghost var lvm_ltmp1, lvm_cM:lvm_code, lvm_ltmp2 := lvm_lemma_block(lvm_b0, lvm_s0, lvm_sN,lvm_ret);
-//   lvm_sM := lvm_ltmp1;
-//   lvm_bM := lvm_ltmp2;
-// //   var lvm_b1:lvm_codes := lvm_get_block(lvm_cM);
-//   assert lvm_sM.ok;
-//   assert lvm_b0.tl == lvm_bM;
-
-//   assert ValidState(lvm_sM);
-//   // assert ValidOperand(lvm_sM,op1);
-//   // assert ValidOperand(lvm_sM,lvm_ret);
-//   // assert OperandContents(lvm_sM,op1) ==  OperandContents(lvm_sM,lvm_ret);
-//   assert evalCode_lax(lvm_cM, lvm_s0, lvm_sM,lvm_ret);
-//   reveal_evalCodeOpaque();
-// }
 
 function method{:opaque} lvm_LOAD(dst:lvm_operand_opr,s:MemState,t:bitWidth,op1:lvm_operand_opr):lvm_code
 {
@@ -299,11 +208,10 @@ function method{:opaque} lvm_LOAD(dst:lvm_operand_opr,s:MemState,t:bitWidth,op1:
 }
 
 
-
 lemma lvm_lemma_Load(lvm_b0:lvm_codes, lvm_s0:lvm_state, lvm_sN:lvm_state,dst:lvm_operand_opr,t:bitWidth,op1:lvm_operand_opr)
   returns (lvm_bM:lvm_codes, lvm_sM:lvm_state)
 //   requires dst.LV?;
-  requires lvm_require(lvm_b0, lvm_LOAD(dst,lvm_s0.m,t,op1), lvm_s0, lvm_sN,dst)
+  requires lvm_require(lvm_b0, lvm_LOAD(dst,lvm_s0.m,t,op1), lvm_s0, lvm_sN)
   requires lvm_is_dst_opr(dst, lvm_s0)
   requires lvm_is_src_opr(op1, lvm_s0)
   requires lvm_get_ok(lvm_s0)
@@ -317,16 +225,18 @@ lemma lvm_lemma_Load(lvm_b0:lvm_codes, lvm_s0:lvm_state, lvm_sN:lvm_state,dst:lv
 //   requires exists d:Data :: Load(lvm_s0.m,lvm_sN.m,OperandContents(lvm_s0,op1).bid,OperandContents(lvm_s0,op1).offset,d);
 
 //   
-  ensures  lvm_ensure(lvm_b0, lvm_bM, lvm_s0, lvm_sM, lvm_sN,dst)
+  ensures  lvm_ensure(lvm_b0, lvm_bM, lvm_s0, lvm_sM, lvm_sN)
   ensures  lvm_get_ok(lvm_sM)
   ensures ValidOperand(lvm_sM,dst);
   ensures  !OperandContents(lvm_sM,dst).Ptr?;
-    ensures  OperandContents(lvm_sM,dst).Int? || OperandContents(lvm_sM,dst).Void?;
+  ensures  OperandContents(lvm_sM,dst).Int? || OperandContents(lvm_sM,dst).Void?;
 
   ensures OperandContents(lvm_sM,dst).Bytes? ==> validBitWidth(|OperandContents(lvm_sM,dst).bytes|)
   ensures OperandContents(lvm_sM,dst).Int? || OperandContents(lvm_sM,dst).Bytes? || OperandContents(lvm_sM,dst).Void?;
   ensures OperandContents(lvm_sM,dst).Int? ==> OperandContents(lvm_sM,dst).itype.size == t;
-//   ensures  lvm_state_eq(lvm_sM,  lvm_s0)
+  ensures  lvm_s0.m == lvm_sM.m;
+    ensures forall d :: ValidOperand(lvm_s0,d) && d != dst ==> ValidOperand(lvm_sM,d) && OperandContents(lvm_s0,d) == OperandContents(lvm_sM,d)
+
 {
   reveal_lvm_LOAD();
   reveal_ValidData();
@@ -335,7 +245,7 @@ lemma lvm_lemma_Load(lvm_b0:lvm_codes, lvm_s0:lvm_state, lvm_sN:lvm_state,dst:lv
   reveal_ValidRegState();
   reveal_ValidData();
 
-  assert evalBlock(lvm_b0, lvm_s0, lvm_sN,dst);
+  assert evalBlock(lvm_b0, lvm_s0, lvm_sN);
   assert lvm_s0.ok;
   assert ValidInstruction(lvm_s0,lvm_b0.hd.ins);
 
@@ -348,24 +258,16 @@ lemma lvm_lemma_Load(lvm_b0:lvm_codes, lvm_s0:lvm_state, lvm_sN:lvm_state,dst:lv
 //   assert lvm_s0.ok == lvm_sN.ok;
   assert d == evalLOAD(lvm_s0.m,lvm_sN.m,lvm_b0.hd.ins.t,OperandContents(lvm_s0,lvm_b0.hd.ins.src));
   assert D(d).D?;
-//   assert evalUpdate(lvm_s0, D(d), evalLOAD(lvm_s0.m,lvm_sN.m,lvm_b0.hd.ins.t,OperandContents(lvm_s0,lvm_b0.hd.ins.src)),lvm_sN);
 
-//   assert exists d:Data :: Load(lvm_s0.m,lvm_sN.m,OperandContents(lvm_s0,lvm_b0.hd.ins.src).bid,OperandContents(lvm_s0,lvm_b0.hd.ins.src).offset,d);
-//   assert dst.LV?;
-//   assert 
-//   assert evalLoad(lvm_s0,dst,OperandContents(lvm_s0,lvm_b0.hd.ins.src).bid,OperandContents(lvm_s0,lvm_b0.hd.ins.src).offset,lvm_sN);
-  
-//   assert evalIns(lvm_b0.hd.ins,lvm_s0,lvm_sN,dst);
-
-  ghost var lvm_ltmp1, lvm_cM:lvm_code, lvm_ltmp2 := lvm_lemma_block(lvm_b0, lvm_s0, lvm_sN,dst);
+  ghost var lvm_ltmp1, lvm_cM:lvm_code, lvm_ltmp2 := lvm_lemma_block(lvm_b0, lvm_s0, lvm_sN);
   lvm_sM := lvm_ltmp1;
   lvm_bM := lvm_ltmp2;
 
   assert lvm_sM.ok;
-  assert  evalCode(lvm_b0.hd, lvm_s0, lvm_sM,dst);
+  assert  evalCode(lvm_b0.hd, lvm_s0, lvm_sM);
   assert lvm_b0.hd == lvm_LOAD(dst,lvm_s0.m,t,op1);
   assert lvm_b0.hd.ins.LOAD?;
-  assert evalIns(lvm_b0.hd.ins,lvm_s0,lvm_sM,dst);
+  assert evalIns(lvm_b0.hd.ins,lvm_s0,lvm_sM);
 
   assert lvm_b0.tl == lvm_bM;
   assert !OperandContents(lvm_sM,dst).Ptr?;
@@ -373,7 +275,7 @@ lemma lvm_lemma_Load(lvm_b0:lvm_codes, lvm_s0:lvm_state, lvm_sN:lvm_state,dst:lv
    assert OperandContents(lvm_sM,dst).Int? ==> OperandContents(lvm_sM,dst).itype.size == t;
 
   assert ValidState(lvm_sM);
-  assert evalCode_lax(lvm_cM, lvm_s0, lvm_sM,dst);
+  assert evalCode_lax(lvm_cM, lvm_s0, lvm_sM);
 }
 
 
@@ -389,7 +291,7 @@ lemma lvm_lemma_Zext(lvm_b0:lvm_codes, lvm_s0:lvm_state, lvm_sN:lvm_state,
             dst:lvm_operand_opr, t:bitWidth,op1:lvm_operand_opr,dstSize:bitWidth)
   returns (lvm_bM:lvm_codes, lvm_sM:lvm_state)
 
-  requires lvm_require(lvm_b0, lvm_code_ZEXT(dst,t,op1,dstSize), lvm_s0, lvm_sN,dst)
+  requires lvm_require(lvm_b0, lvm_code_ZEXT(dst,t,op1,dstSize), lvm_s0, lvm_sN)
   requires lvm_is_dst_opr(dst, lvm_s0)
   requires lvm_is_src_opr(op1, lvm_s0)
   requires lvm_get_ok(lvm_s0)
@@ -404,7 +306,7 @@ lemma lvm_lemma_Zext(lvm_b0:lvm_codes, lvm_s0:lvm_state, lvm_sN:lvm_state,
 //   requires !OperandContents(lvm_s0,dst).itype.signed;
 
 // //   
-  ensures  lvm_ensure(lvm_b0, lvm_bM, lvm_s0, lvm_sM, lvm_sN,dst)
+  ensures  lvm_ensure(lvm_b0, lvm_bM, lvm_s0, lvm_sM, lvm_sN)
   ensures  lvm_get_ok(lvm_sM)
   ensures  ValidOperand(lvm_sM,dst)
   ensures  OperandContents(lvm_sM,dst).Int?;
@@ -412,6 +314,8 @@ lemma lvm_lemma_Zext(lvm_b0:lvm_codes, lvm_s0:lvm_state, lvm_sN:lvm_state,
   ensures  OperandContents(lvm_sM,dst).itype.size == dstSize;
   ensures OperandContents(lvm_sM, dst).val == evalZEXT(OperandContents(lvm_s0,op1),dstSize).val;
   ensures  lvm_state_eq(lvm_sM, lvm_update_ok(lvm_sM, lvm_update_all( lvm_sM, lvm_s0)))
+  ensures lvm_s0.m == lvm_sM.m;
+    ensures forall d :: ValidOperand(lvm_s0,d) && d != dst ==> ValidOperand(lvm_sM,d) && OperandContents(lvm_s0,d) == OperandContents(lvm_sM,d)
 
 {
     reveal_lvm_code_ZEXT();
@@ -421,23 +325,19 @@ lemma lvm_lemma_Zext(lvm_b0:lvm_codes, lvm_s0:lvm_state, lvm_sN:lvm_state,
 
     assert ValidInstruction(lvm_s0, lvm_code_ZEXT(dst,t,op1,dstSize).ins);
 
-    ghost var lvm_ltmp1, lvm_cM:lvm_code, lvm_ltmp2 := lvm_lemma_block(lvm_b0, lvm_s0, lvm_sN,dst);
+    ghost var lvm_ltmp1, lvm_cM:lvm_code, lvm_ltmp2 := lvm_lemma_block(lvm_b0, lvm_s0, lvm_sN);
     lvm_sM := lvm_ltmp1;
     lvm_bM := lvm_ltmp2;
     // assert lvm_b0.tl == lvm_bM;
     assert ValidState(lvm_s0);
     // assert lvm_s0.ok;
     assert ValidState(lvm_sM);
-    // assert ValidOperand(lvm_sM,dst);
-    // assert evalIns(lvm_code_Add(dst, size,src1,src2).ins,lvm_s0,lvm_sM,dst);
-    // assert evalUpdate(lvm_s0, dst, evalADD(OperandContents(lvm_s0,dst).itype.size,OperandContents(lvm_s0,src1),OperandContents(lvm_s0,src2)),lvm_sM);
-    // assert ValidData(lvm_sM,evalADD(OperandContents(lvm_s0,dst).itype.size,OperandContents(lvm_s0,src1),OperandContents(lvm_s0,src2)));
-    // assert OperandContents(lvm_sM, dst).val == evalADD(OperandContents(lvm_s0,dst).itype.size,OperandContents(lvm_s0,src1),OperandContents(lvm_s0,src2)).val;
+    
   assert lvm_sM.ok;
   assert lvm_b0.tl == lvm_bM;
 
   assert ValidState(lvm_sM);
-  assert evalCode_lax(lvm_cM, lvm_s0, lvm_sM,dst);
+  assert evalCode_lax(lvm_cM, lvm_s0, lvm_sM);
   reveal_evalCodeOpaque();
 }
 
@@ -453,7 +353,7 @@ lemma lvm_lemma_Sext(lvm_b0:lvm_codes, lvm_s0:lvm_state, lvm_sN:lvm_state,
             dst:lvm_operand_opr, t:bitWidth,op1:lvm_operand_opr,dstSize:bitWidth)
   returns (lvm_bM:lvm_codes, lvm_sM:lvm_state)
 
-  requires lvm_require(lvm_b0, lvm_code_SEXT(dst,t,op1,dstSize), lvm_s0, lvm_sN,dst)
+  requires lvm_require(lvm_b0, lvm_code_SEXT(dst,t,op1,dstSize), lvm_s0, lvm_sN)
   requires lvm_is_dst_opr(dst, lvm_s0)
   requires lvm_is_src_opr(op1, lvm_s0)
   requires lvm_get_ok(lvm_s0)
@@ -468,7 +368,7 @@ lemma lvm_lemma_Sext(lvm_b0:lvm_codes, lvm_s0:lvm_state, lvm_sN:lvm_state,
 //   requires !OperandContents(lvm_s0,dst).itype.signed;
 
 // //   
-  ensures  lvm_ensure(lvm_b0, lvm_bM, lvm_s0, lvm_sM, lvm_sN,dst)
+  ensures  lvm_ensure(lvm_b0, lvm_bM, lvm_s0, lvm_sM, lvm_sN)
   ensures  lvm_get_ok(lvm_sM)
   ensures  ValidOperand(lvm_sM,dst)
   ensures  OperandContents(lvm_sM,dst).Int?;
@@ -476,6 +376,7 @@ lemma lvm_lemma_Sext(lvm_b0:lvm_codes, lvm_s0:lvm_state, lvm_sN:lvm_state,
   ensures  OperandContents(lvm_sM,dst).itype.size == dstSize;
   ensures OperandContents(lvm_sM, dst).val == evalSEXT(OperandContents(lvm_s0,op1),dstSize).val;
   ensures  lvm_state_eq(lvm_sM, lvm_update_ok(lvm_sM, lvm_update_all( lvm_sM, lvm_s0)))
+    ensures forall d :: ValidOperand(lvm_s0,d) && d != dst ==> ValidOperand(lvm_sM,d) && OperandContents(lvm_s0,d) == OperandContents(lvm_sM,d)
 
 {
     reveal_lvm_code_SEXT();
@@ -485,23 +386,19 @@ lemma lvm_lemma_Sext(lvm_b0:lvm_codes, lvm_s0:lvm_state, lvm_sN:lvm_state,
 
     assert ValidInstruction(lvm_s0, lvm_code_SEXT(dst,t,op1,dstSize).ins);
 
-    ghost var lvm_ltmp1, lvm_cM:lvm_code, lvm_ltmp2 := lvm_lemma_block(lvm_b0, lvm_s0, lvm_sN,dst);
+    ghost var lvm_ltmp1, lvm_cM:lvm_code, lvm_ltmp2 := lvm_lemma_block(lvm_b0, lvm_s0, lvm_sN);
     lvm_sM := lvm_ltmp1;
     lvm_bM := lvm_ltmp2;
     // assert lvm_b0.tl == lvm_bM;
     assert ValidState(lvm_s0);
     // assert lvm_s0.ok;
     assert ValidState(lvm_sM);
-    // assert ValidOperand(lvm_sM,dst);
-    // assert evalIns(lvm_code_Add(dst, size,src1,src2).ins,lvm_s0,lvm_sM,dst);
-    // assert evalUpdate(lvm_s0, dst, evalADD(OperandContents(lvm_s0,dst).itype.size,OperandContents(lvm_s0,src1),OperandContents(lvm_s0,src2)),lvm_sM);
-    // assert ValidData(lvm_sM,evalADD(OperandContents(lvm_s0,dst).itype.size,OperandContents(lvm_s0,src1),OperandContents(lvm_s0,src2)));
-    // assert OperandContents(lvm_sM, dst).val == evalADD(OperandContents(lvm_s0,dst).itype.size,OperandContents(lvm_s0,src1),OperandContents(lvm_s0,src2)).val;
+   
   assert lvm_sM.ok;
   assert lvm_b0.tl == lvm_bM;
 
   assert ValidState(lvm_sM);
-  assert evalCode_lax(lvm_cM, lvm_s0, lvm_sM,dst);
+  assert evalCode_lax(lvm_cM, lvm_s0, lvm_sM);
   reveal_evalCodeOpaque();
 }
 
@@ -516,7 +413,7 @@ lemma lvm_lemma_Shl(lvm_b0:lvm_codes, lvm_s0:lvm_state, lvm_sN:lvm_state,
             dst:lvm_operand_opr, src:lvm_operand_opr,shiftAmt:lvm_operand_opr)
   returns (lvm_bM:lvm_codes, lvm_sM:lvm_state)
 
-  requires lvm_require(lvm_b0, lvm_code_SHL(dst,src,shiftAmt), lvm_s0, lvm_sN,dst)
+  requires lvm_require(lvm_b0, lvm_code_SHL(dst,src,shiftAmt), lvm_s0, lvm_sN)
   requires lvm_is_dst_opr(dst, lvm_s0)
   requires lvm_is_src_opr(src, lvm_s0)
   requires lvm_get_ok(lvm_s0)
@@ -533,7 +430,7 @@ lemma lvm_lemma_Shl(lvm_b0:lvm_codes, lvm_s0:lvm_state, lvm_sN:lvm_state,
   requires OperandContents(lvm_s0,shiftAmt).val > 0
   requires OperandContents(lvm_s0,dst).itype.signed == OperandContents(lvm_s0,src).itype.signed
 // //   
-  ensures  lvm_ensure(lvm_b0, lvm_bM, lvm_s0, lvm_sM, lvm_sN,dst)
+  ensures  lvm_ensure(lvm_b0, lvm_bM, lvm_s0, lvm_sM, lvm_sN)
   ensures  lvm_get_ok(lvm_sM)
   ensures  ValidOperand(lvm_sM,dst)
   ensures  ValidOperand(lvm_sM,src)
@@ -545,6 +442,8 @@ lemma lvm_lemma_Shl(lvm_b0:lvm_codes, lvm_s0:lvm_state, lvm_sN:lvm_state,
   ensures OperandContents(lvm_sM,dst).itype.signed == OperandContents(lvm_sM,src).itype.signed
   ensures OperandContents(lvm_sM, dst) == evalSHL(OperandContents(lvm_s0,src),OperandContents(lvm_s0,shiftAmt));
   ensures  lvm_state_eq(lvm_sM, lvm_update_ok(lvm_sM, lvm_update_all( lvm_sM, lvm_s0)))
+  ensures lvm_s0.m == lvm_sM.m;
+    ensures forall d :: ValidOperand(lvm_s0,d) && d != dst ==> ValidOperand(lvm_sM,d) && OperandContents(lvm_s0,d) == OperandContents(lvm_sM,d)
 
 {
     reveal_lvm_code_SHL();
@@ -554,7 +453,7 @@ lemma lvm_lemma_Shl(lvm_b0:lvm_codes, lvm_s0:lvm_state, lvm_sN:lvm_state,
 
     assert ValidInstruction(lvm_s0, lvm_code_SHL(dst,src,shiftAmt).ins);
 
-    ghost var lvm_ltmp1, lvm_cM:lvm_code, lvm_ltmp2 := lvm_lemma_block(lvm_b0, lvm_s0, lvm_sN,dst);
+    ghost var lvm_ltmp1, lvm_cM:lvm_code, lvm_ltmp2 := lvm_lemma_block(lvm_b0, lvm_s0, lvm_sN);
     lvm_sM := lvm_ltmp1;
     lvm_bM := lvm_ltmp2;
     assert ValidState(lvm_s0);
@@ -564,25 +463,83 @@ lemma lvm_lemma_Shl(lvm_b0:lvm_codes, lvm_s0:lvm_state, lvm_sN:lvm_state,
     assert lvm_b0.tl == lvm_bM;
 
     assert ValidState(lvm_sM);
-    assert evalCode_lax(lvm_cM, lvm_s0, lvm_sM,dst);
+    assert evalCode_lax(lvm_cM, lvm_s0, lvm_sM);
     reveal_evalCodeOpaque();
 }
 
+function method{:opaque} lvm_code_ICMP(dst:lvm_operand_opr,cond:lvm_cond,size:nat,op1:lvm_operand_opr,op2:lvm_operand_opr):(out:lvm_code)
+{
+    reveal_IntFits();
+    Ins(ICMP(dst,cond,size,op1,op2))
+}
+
+lemma lvm_lemma_Icmp(lvm_b0:lvm_codes, lvm_s0:lvm_state, lvm_sN:lvm_state,
+                    dst:lvm_operand_opr,cond:lvm_cond,size:nat,op1:lvm_operand_opr,op2:lvm_operand_opr)
+  returns (lvm_bM:lvm_codes, lvm_sM:lvm_state)
+  requires lvm_require(lvm_b0, lvm_code_ICMP(dst,cond,size,op1,op2), lvm_s0, lvm_sN)
+  requires lvm_is_dst_opr(dst, lvm_s0)
+  requires lvm_is_src_opr(op1, lvm_s0)
+  requires lvm_get_ok(lvm_s0)
+
+  requires lvm_code_ICMP(dst,cond,size,op1,op2).Ins?;
+  // requires ValidInstruction(lvm_s0,lvm_code_ICMP(dst,cond,size,op1,op2).ins);
+  requires ValidOperand(lvm_s0,dst) && ValidOperand(lvm_s0,op1) && ValidOperand(lvm_s0,op2);
+  requires OperandContents(lvm_s0,op1).Int?;
+  requires OperandContents(lvm_s0,op2).Int?;
+  requires typesMatch(OperandContents(lvm_s0,op1),OperandContents(lvm_s0,op2));
+  requires size == OperandContents(lvm_s0,op1).itype.size
+
+  ensures  lvm_ensure(lvm_b0, lvm_bM, lvm_s0, lvm_sM, lvm_sN)
+  ensures  lvm_get_ok(lvm_sM)
+  ensures  ValidOperand(lvm_sM,dst)
+  ensures  ValidOperand(lvm_sM,op1)
+  ensures  OperandContents(lvm_sM,dst).Int?;
+  ensures  OperandContents(lvm_sM,op1).Int?;
+  ensures OperandContents(lvm_s0,op1).itype == OperandContents(lvm_sM,op1).itype;
+
+  // ensures OperandContents(lvm_sM,dst).itype.size == OperandContents(lvm_sM,src).itype.size 
+  // ensures OperandContents(lvm_sM,dst).itype.signed == OperandContents(lvm_sM,src).itype.signed
+  ensures OperandContents(lvm_sM, dst) == evalICMP(cond,size,OperandContents(lvm_s0,op1),OperandContents(lvm_s0,op2));
+  ensures  lvm_state_eq(lvm_sM, lvm_update_ok(lvm_sM, lvm_update_all( lvm_sM, lvm_s0)))
+  ensures forall d :: ValidOperand(lvm_s0,d) && d != dst ==> ValidOperand(lvm_sM,d) && OperandContents(lvm_s0,d) == OperandContents(lvm_sM,d)
+
+{
+    reveal_lvm_code_ICMP();
+    reveal_eval_code();
+    reveal_evalCodeOpaque();
+
+    assert lvm_code_ICMP(dst,cond,size,op1,op2).Ins?;
+    assert ValidInstruction(lvm_s0,lvm_code_ICMP(dst,cond,size,op1,op2).ins);
+
+    ghost var lvm_ltmp1, lvm_cM:lvm_code, lvm_ltmp2 := lvm_lemma_block(lvm_b0, lvm_s0, lvm_sN);
+    lvm_sM := lvm_ltmp1;
+    lvm_bM := lvm_ltmp2;
+    assert ValidState(lvm_s0);
+    assert ValidState(lvm_sM);
+  
+    assert lvm_sM.ok;
+    assert lvm_b0.tl == lvm_bM;
+
+    assert ValidState(lvm_sM);
+    assert evalCode_lax(lvm_cM, lvm_s0, lvm_sM);
+    reveal_evalCodeOpaque();
+
+}
 
 function method{:opaque} lvm_code_Empty():lvm_code
 {   
     lvm_Block(lvm_CNil())
 }       
 
-lemma lvm_lemma_Empty(lvm_b0:lvm_codes, lvm_s0:lvm_state, lvm_sN:lvm_state,o:operand)
+lemma lvm_lemma_Empty(lvm_b0:lvm_codes, lvm_s0:lvm_state, lvm_sN:lvm_state)
   returns (lvm_bM:lvm_codes, lvm_sM:lvm_state)
-  requires lvm_require(lvm_b0, lvm_code_Empty(), lvm_s0, lvm_sN,o)
+  requires lvm_require(lvm_b0, lvm_code_Empty(), lvm_s0, lvm_sN)
   requires lvm_get_ok(lvm_s0)
-  ensures  lvm_ensure(lvm_b0, lvm_bM, lvm_s0, lvm_sM, lvm_sN,o)
+  ensures  lvm_ensure(lvm_b0, lvm_bM, lvm_s0, lvm_sM, lvm_sN)
   ensures  lvm_get_ok(lvm_sM) // ValidState(sM)
   ensures  lvm_state_eq(lvm_sM, lvm_s0)
   ensures  lvm_state_eq(lvm_sM, lvm_update_mem( lvm_sM, lvm_update_ok(lvm_sM, lvm_sM)))
-  ensures  forall s2 :: evalCode(lvm_b0.hd, lvm_s0, s2,o) ==> s2.ok 
+  ensures  forall s2 :: evalCode(lvm_b0.hd, lvm_s0, s2) ==> s2.ok 
 {
     reveal_lvm_code_Empty();
     reveal_eval_code();
@@ -597,15 +554,13 @@ lemma lvm_lemma_Empty(lvm_b0:lvm_codes, lvm_s0:lvm_state, lvm_sN:lvm_state,o:ope
     assert lvm_code_Empty().block.CNil?;
     assert lvm_b0.hd.Block?;
     assert lvm_get_block(lvm_b0.hd).CNil?;
-    assert evalBlock(lvm_get_block(lvm_b0.hd),lvm_s0, lvm_s0,o);
-    assert forall r :: r == lvm_s0 ==> eval_code(lvm_b0.hd,lvm_s0,r,o);
-    assert evalCode_lax(Block(lvm_b0), lvm_s0, lvm_sN, o);
+    assert evalBlock(lvm_get_block(lvm_b0.hd),lvm_s0, lvm_s0);
+    assert forall r :: r == lvm_s0 ==> eval_code(lvm_b0.hd,lvm_s0,r);
+    assert evalCode_lax(Block(lvm_b0), lvm_s0, lvm_sN);
 
-    assert evalBlock(lvm_b0, lvm_s0, lvm_sN,o) ==> exists r' :: evalCode(lvm_b0.hd, lvm_s0, r',o) && evalBlock(lvm_b0.tl, r', lvm_sN,o);
-    assert exists r' :: if evalCode(lvm_b0.hd, lvm_s0, r',o) then true else true;
 
     // lvm_sM := lvm_lemma_empty(lvm_s0,lvm_sN);
-    ghost var lvm_ltmp1, lvm_cM:lvm_code, lvm_ltmp2 := lvm_lemma_block(lvm_b0, lvm_s0, lvm_sN,o);
+    ghost var lvm_ltmp1, lvm_cM:lvm_code, lvm_ltmp2 := lvm_lemma_block(lvm_b0, lvm_s0, lvm_sN);
     lvm_sM := lvm_ltmp1;
     lvm_bM := lvm_ltmp2;
     var lvm_b1:lvm_codes := lvm_get_block(lvm_cM);
