Dafny/examples/sextChallengeProblem1Simplified.i.dfy
@@ -82,7 +82,7 @@ requires IsValidBid(lvm_s0.m,op1.d.bid) ==> op1.d.offset + ((Int(2,IntType(8,fal
   ensures  !OperandContents(lvm_sM, dst).Void? ==> lvm_state_eq(lvm_sM, lvm_update_ok(lvm_sM, lvm_update_mem( lvm_sM, lvm_s0)))
 {
   reveal_lvm_simple_challenge1_cont();
-  reveal_lvm_RET();
+  reveal_lvm_code_Ret();
   reveal_lvm_LOAD();
   reveal_lvm_code_Add();
   reveal_lvm_code_SEXT();
