Dafny/examples/simple.i.dfy
@@ -35,10 +35,10 @@ function method{:opaque} lvm_code_Add_single(dst:lvm_operand_opr, size:nat, src1
 }
 
 lemma lvm_lemma_Add_single(lvm_b0:lvm_codes, lvm_s0:lvm_state, lvm_sN:lvm_state, 
-            dst:lvm_operand_opr, size:nat, src1:lvm_operand_opr,src2:lvm_operand_opr,o:operand)
+            dst:lvm_operand_opr, size:nat, src1:lvm_operand_opr,src2:lvm_operand_opr)
   returns (lvm_bM:lvm_codes, lvm_sM:lvm_state)
   requires src1.D?;
-  requires lvm_require(lvm_b0, lvm_code_Add_single(dst, size,src1), lvm_s0, lvm_sN,dst)
+  requires lvm_require(lvm_b0, lvm_code_Add_single(dst, size,src1), lvm_s0, lvm_sN)
   requires lvm_is_dst_opr(dst, lvm_s0)
   requires lvm_is_src_opr(src1, lvm_s0)
   requires lvm_get_ok(lvm_s0)
@@ -48,7 +48,7 @@ lemma lvm_lemma_Add_single(lvm_b0:lvm_codes, lvm_s0:lvm_state, lvm_sN:lvm_state,
   requires lvm_code_Add_single(dst, size,src1).Ins?;
   requires ValidOperand(lvm_s0,dst)
 //   
-  ensures  lvm_ensure(lvm_b0, lvm_bM, lvm_s0, lvm_sM, lvm_sN,dst)
+  ensures  lvm_ensure(lvm_b0, lvm_bM, lvm_s0, lvm_sM, lvm_sN)
   ensures  lvm_get_ok(lvm_sM)
   ensures  ValidOperand(lvm_sM,dst)
   ensures  OperandContents(lvm_sM,dst).Int?;
@@ -57,7 +57,7 @@ lemma lvm_lemma_Add_single(lvm_b0:lvm_codes, lvm_s0:lvm_state, lvm_sN:lvm_state,
   evalADD(OperandContents(lvm_s0,dst).itype.size,OperandContents(lvm_s0,src1),D(Int(4,src1.d.itype)).d).val;
   ensures  OperandContents(lvm_sM, dst).val == OperandContents(lvm_s0, dst).val + 4
   ensures  lvm_state_eq(lvm_sM, lvm_update_ok(lvm_sM, lvm_update_all( lvm_sM, lvm_s0)))
-  ensures  forall s2 :: evalCode(lvm_b0.hd, lvm_s0, s2,o) ==> s2.ok
+  ensures  forall s2 :: evalCode(lvm_b0.hd, lvm_s0, s2) ==> s2.ok
 
 {
     reveal_lvm_code_Add_single();
@@ -69,13 +69,13 @@ lemma lvm_lemma_Add_single(lvm_b0:lvm_codes, lvm_s0:lvm_state, lvm_sN:lvm_state,
     assert ValidState(lvm_s0);
     assert lvm_b0.hd.Ins?;
     var lvm_old_s:lvm_state := lvm_s0;
-    ghost var lvm_ltmp1, lvm_cM:lvm_code, lvm_ltmp2 := lvm_lemma_block(lvm_b0, lvm_s0, lvm_sN,dst);
+    ghost var lvm_ltmp1, lvm_cM:lvm_code, lvm_ltmp2 := lvm_lemma_block(lvm_b0, lvm_s0, lvm_sN);
     lvm_sM := lvm_ltmp1;
     lvm_bM := lvm_ltmp2;
     assert lvm_b0.tl == lvm_bM;
     assert lvm_bM.CNil?;
 
-    assert evalCode_lax(lvm_cM, lvm_s0, lvm_sM,dst);
+    assert evalCode_lax(lvm_cM, lvm_s0, lvm_sM);
     assert OperandContents(lvm_sM, dst).val == OperandContents(lvm_s0, dst).val + 4;
 
     reveal_evalCodeOpaque();
@@ -104,11 +104,11 @@ function method {:opaque} lvm_code_Add_Multiple(dst:lvm_operand_opr, size:nat, s
 }
 
 lemma lvm_lemma_Add_Multiple(lvm_b0:lvm_codes, lvm_s0:lvm_state, lvm_sN:lvm_state, 
-            dst:lvm_operand_opr, size:nat, src1:lvm_operand_opr,src2:lvm_operand_opr,o:operand)
+            dst:lvm_operand_opr, size:nat, src1:lvm_operand_opr,src2:lvm_operand_opr)
   returns (lvm_bM:lvm_codes, lvm_sM:lvm_state)
   requires src1.D?;
   requires src1.d.Int?;
-  requires lvm_require(lvm_b0, lvm_code_Add_Multiple(dst, size,src1), lvm_s0, lvm_sN,dst)
+  requires lvm_require(lvm_b0, lvm_code_Add_Multiple(dst, size,src1), lvm_s0, lvm_sN)
   requires lvm_is_dst_opr(dst, lvm_s0)
   requires lvm_is_src_opr(src1, lvm_s0)
   requires lvm_get_ok(lvm_s0)
@@ -121,7 +121,7 @@ lemma lvm_lemma_Add_Multiple(lvm_b0:lvm_codes, lvm_s0:lvm_state, lvm_sN:lvm_stat
 
   requires ValidOperand(lvm_s0,dst)
 //   
-  ensures  lvm_ensure(lvm_b0, lvm_bM, lvm_s0, lvm_sM, lvm_sN,dst)
+  ensures  lvm_ensure(lvm_b0, lvm_bM, lvm_s0, lvm_sM, lvm_sN)
   ensures  lvm_get_ok(lvm_sM) 
   ensures ValidOperand(lvm_sM,dst)
   ensures OperandContents(lvm_sM,dst).Int?;
@@ -136,16 +136,16 @@ lemma lvm_lemma_Add_Multiple(lvm_b0:lvm_codes, lvm_s0:lvm_state, lvm_sN:lvm_stat
     reveal_eval_code();
     reveal_evalCodeOpaque();
     reveal_lvm_code_Add();
-    reveal_lvm_RET();
+    reveal_lvm_code_Ret();
 
     assert lvm_code_Add_Multiple(dst, size,src1).block.hd.Ins?;
 
     assert ValidState(lvm_s0);
     var lvm_old_s:lvm_state := lvm_s0;
-    assert evalCode(lvm_Block(lvm_b0), lvm_s0, lvm_sN,dst);
-    assert eval_code(lvm_Block(lvm_b0), lvm_s0, lvm_sN,dst);
+    assert evalCode(lvm_Block(lvm_b0), lvm_s0, lvm_sN);
+    assert eval_code(lvm_Block(lvm_b0), lvm_s0, lvm_sN);
 
-    ghost var lvm_ltmp1, lvm_cM:lvm_code, lvm_ltmp2 := lvm_lemma_block(lvm_b0, lvm_s0, lvm_sN,dst);
+    ghost var lvm_ltmp1, lvm_cM:lvm_code, lvm_ltmp2 := lvm_lemma_block(lvm_b0, lvm_s0, lvm_sN);
     lvm_sM := lvm_ltmp1;
     lvm_bM := lvm_ltmp2;
     var lvm_b1:lvm_codes := lvm_get_block(lvm_cM);
@@ -155,30 +155,30 @@ lemma lvm_lemma_Add_Multiple(lvm_b0:lvm_codes, lvm_s0:lvm_state, lvm_sN:lvm_stat
     assert val.d.Int?;
     assert lvm_b1.hd == lvm_code_Add(dst, size,src1,val);
     assert ValidState(lvm_s0);
-    assert evalCode_lax(lvm_Block(lvm_b1), lvm_s0, lvm_sM,dst);
+    assert evalCode_lax(lvm_Block(lvm_b1), lvm_s0, lvm_sM);
     assert OperandContents(lvm_s0,dst).Int?;
 
     // assert evalUpdate(lvm_s0, dst, evalADD(size,OperandContents(lvm_s0,src1),OperandContents(lvm_s0,val)),lvm_sM);
-    assert evalCode(lvm_Block(lvm_b1), lvm_s0, lvm_sM,dst);
-    assert evalBlock(lvm_Block(lvm_b1).block, lvm_s0, lvm_sM,dst);
+    assert evalCode(lvm_Block(lvm_b1), lvm_s0, lvm_sM);
+    assert evalBlock(lvm_Block(lvm_b1).block, lvm_s0, lvm_sM);
     assert lvm_Block(lvm_b1).block.hd == Ins(ADD(dst, size,src1,val));
-    assert  exists r' ::  evalCode(lvm_b1.hd, lvm_s0, r',dst);
-    assert  exists r' ::  evalIns(lvm_b1.hd.ins, lvm_s0, r',dst);
+    assert  exists r' ::  evalCode(lvm_b1.hd, lvm_s0, r');
+    assert  exists r' ::  evalIns(lvm_b1.hd.ins, lvm_s0, r');
 
     var val2 := D(Int(5,src1.d.itype));
     var step1 := evalADD(OperandContents(lvm_s0,dst).itype.size,OperandContents(lvm_s0,src1),val.d);
 
 
-    ghost var lvm_b2, lvm_s2 := lvm_lemma_Add(lvm_b1, lvm_s0, lvm_sM, dst, size,src1,val,o);
+    ghost var lvm_b2, lvm_s2 := lvm_lemma_Add(lvm_b1, lvm_s0, lvm_sM, dst, size,src1,val);
 
 
     assert OperandContents(lvm_s2, dst).val == step1.val;
     assert OperandContents(lvm_s0, src1) == OperandContents(lvm_s2, src1); 
 
-    assert  lvm_require(lvm_b2, lvm_code_Add(dst, size,src1,val2), lvm_s2, lvm_sM,dst);
+    assert  lvm_require(lvm_b2, lvm_code_Add(dst, size,src1,val2), lvm_s2, lvm_sM);
     var step2 := evalADD(OperandContents(lvm_s2,dst).itype.size,OperandContents(lvm_s2,src1),val2.d);
 
-    ghost var lvm_b3, lvm_s3 := lvm_lemma_Add(lvm_b2, lvm_s2, lvm_sM, dst, size,src1,val2,o);
+    ghost var lvm_b3, lvm_s3 := lvm_lemma_Add(lvm_b2, lvm_s2, lvm_sM, dst, size,src1,val2);
     assert OperandContents(lvm_s3, dst).val 
         == evalADD(OperandContents(lvm_s2,dst).itype.size,OperandContents(lvm_s2,src1),val2.d).val;
   
@@ -189,23 +189,22 @@ lemma lvm_lemma_Add_Multiple(lvm_b0:lvm_codes, lvm_s0:lvm_state, lvm_sN:lvm_stat
     
     ghost var lvm_b4, lvm_s4 := lvm_lemma_Ret(lvm_b3, lvm_s3, lvm_sM, dst, D(Void));
     assert lvm_b4.CNil?;
-    assert eval_code(lvm_Block(lvm_b4), lvm_s4, lvm_sM,dst);
+    assert eval_code(lvm_Block(lvm_b4), lvm_s4, lvm_sM);
     lvm_sM := lvm_lemma_empty(lvm_s4,lvm_sM);
     assert   OperandContents(lvm_sM, dst).val  == step2.val;
 
-    assert evalCode_lax(lvm_cM, lvm_s0, lvm_sM,dst);
+    assert evalCode_lax(lvm_cM, lvm_s0, lvm_sM);
     assert OperandContents(lvm_s0, src1) == OperandContents(lvm_sM, src1); 
 
     assert OperandContents(lvm_sM, dst).val == step2.val;
     assert  OperandContents(lvm_sM, dst).val == evalADD(OperandContents(lvm_s0,dst).itype.size,OperandContents(lvm_s0,src1),val2.d).val;
     assert ValidState(lvm_sM);
-
     reveal_evalCodeOpaque();
 }
 
 
 
-////
+// ////
 
 function method {:opaque} lvm_code_Add_Multiple1(dst:lvm_operand_opr, size:nat, src1:lvm_operand_opr, src2:lvm_operand_opr): (out:lvm_code)
     requires src1.D?;
@@ -234,13 +233,13 @@ function method {:opaque} lvm_code_Add_Multiple1(dst:lvm_operand_opr, size:nat, 
 }
 
 lemma lvm_lemma_Add_Multiple1(lvm_b0:lvm_codes, lvm_s0:lvm_state, lvm_sN:lvm_state, 
-            dst:lvm_operand_opr, size:nat, src1:lvm_operand_opr,src2:lvm_operand_opr,o:operand)
+            dst:lvm_operand_opr, size:nat, src1:lvm_operand_opr,src2:lvm_operand_opr)
   returns (lvm_bM:lvm_codes, lvm_sM:lvm_state)
   requires src1.D?;
   requires src1.d.Int?;
   requires src2.D?;
   requires src2.d.Int?;
-  requires lvm_require(lvm_b0, lvm_code_Add_Multiple1(dst, size,src1,src2), lvm_s0, lvm_sN,dst)
+  requires lvm_require(lvm_b0, lvm_code_Add_Multiple1(dst, size,src1,src2), lvm_s0, lvm_sN)
   requires lvm_is_dst_opr(dst, lvm_s0)
   requires lvm_is_dst_opr(src2, lvm_s0)
   requires lvm_is_src_opr(src1, lvm_s0)
@@ -253,31 +252,31 @@ lemma lvm_lemma_Add_Multiple1(lvm_b0:lvm_codes, lvm_s0:lvm_state, lvm_sN:lvm_sta
   requires ValidOperand(lvm_s0,dst);
   requires OperandContents(lvm_s0,dst).Int?;
 //   
-  ensures  lvm_ensure(lvm_b0, lvm_bM, lvm_s0, lvm_sM, lvm_sN,dst)
+  ensures  lvm_ensure(lvm_b0, lvm_bM, lvm_s0, lvm_sM, lvm_sN)
   ensures  lvm_get_ok(lvm_sM) 
   ensures ValidOperand(lvm_sM,dst)
   ensures OperandContents(lvm_sM,dst).Int?;
   ensures OperandContents(lvm_s0,dst).Int?;
 
-  // ensures  OperandContents(lvm_sM, dst).val == evalADD(OperandContents(lvm_s0,dst).itype.size,OperandContents(lvm_s0,src1),D(Int(5,src1.d.itype)).d).val;
-  ensures ToTwosComp(OperandContents(lvm_sM, dst)).val == 
-          (OperandContents(lvm_s0, src1).val + D(Int(5,src1.d.itype)).d.val + D(Int(4,src1.d.itype)).d.val ) % Pow256(OperandContents(lvm_s0, src1).itype.size)
+  ensures OperandContents(lvm_sM, dst).val == evalADD(OperandContents(lvm_s0,dst).itype.size,OperandContents(lvm_s0,src2),D(Int(5,src2.d.itype)).d).val
+  // ensures ToTwosComp(OperandContents(lvm_sM, dst)).val == 
+          // (OperandContents(lvm_s0, src1).val + D(Int(5,src1.d.itype)).d.val + D(Int(4,src1.d.itype)).d.val ) % Pow256(OperandContents(lvm_s0, src1).itype.size)
   ensures  lvm_state_eq(lvm_sM, lvm_update_ok(lvm_sM, lvm_update_all( lvm_sM, lvm_s0)))
 {
     reveal_lvm_code_Add_Multiple1();
     reveal_eval_code();
     reveal_evalCodeOpaque();
     reveal_lvm_code_Add();
-      reveal_lvm_RET();
+      reveal_lvm_code_Ret();
 
     assert lvm_code_Add_Multiple1(dst, size,src1,src2).block.hd.Ins?;
 
     assert ValidState(lvm_s0);
     var lvm_old_s:lvm_state := lvm_s0;
-    assert evalCode(lvm_Block(lvm_b0), lvm_s0, lvm_sN,dst);
-    assert eval_code(lvm_Block(lvm_b0), lvm_s0, lvm_sN,dst);
+    assert evalCode(lvm_Block(lvm_b0), lvm_s0, lvm_sN);
+    assert eval_code(lvm_Block(lvm_b0), lvm_s0, lvm_sN);
 
-    ghost var lvm_ltmp1, lvm_cM:lvm_code, lvm_ltmp2 := lvm_lemma_block(lvm_b0, lvm_s0, lvm_sN,dst);
+    ghost var lvm_ltmp1, lvm_cM:lvm_code, lvm_ltmp2 := lvm_lemma_block(lvm_b0, lvm_s0, lvm_sN);
     lvm_sM := lvm_ltmp1;
     lvm_bM := lvm_ltmp2;
     var lvm_b1:lvm_codes := lvm_get_block(lvm_cM);
@@ -299,37 +298,35 @@ lemma lvm_lemma_Add_Multiple1(lvm_b0:lvm_codes, lvm_s0:lvm_state, lvm_sN:lvm_sta
       assert lvm_b1.hd.ins.dst == src2;
       assert lvm_Block(lvm_b1).block.hd == Ins(ADD(src2, size,src1,val));
       // assert  exists r' ::  evalCode(lvm_b1.hd, lvm_s0, r',src2);
-        assert evalCode(lvm_Block(lvm_b1), lvm_s0, lvm_sM,dst);
+        assert evalCode(lvm_Block(lvm_b1), lvm_s0, lvm_sM);
 
-    // assert  exists r' ::  evalIns(lvm_b1.hd.ins, lvm_s0, r',src2);
-      // assert  evalIns(lvm_b1.hd.ins, lvm_s0, lvm_sM,dst);
-
-      // assert exists r' :: evalCode(lvm_b1.hd, lvm_s0, r',dst);
-
-      assert evalBlock(lvm_b1,lvm_s0, lvm_sM,dst);
-      assert evalCode(lvm_Block(lvm_b1), lvm_s0, lvm_sM,dst);
-      assert  exists r' ::  evalCode(lvm_b1.hd, lvm_s0, r',dst);
-      assert  exists r' ::  evalIns(lvm_b1.hd.ins, lvm_s0, r',dst); // ???  
+      assert evalBlock(lvm_b1,lvm_s0, lvm_sM);
+      assert evalCode(lvm_Block(lvm_b1), lvm_s0, lvm_sM);
+      assert  exists r' ::  evalCode(lvm_b1.hd, lvm_s0, r');
+      assert  exists r' ::  evalIns(lvm_b1.hd.ins, lvm_s0, r'); // ???  
 
     var val2 := D(Int(5,src2.d.itype));
     var step1 := evalADD(OperandContents(lvm_s0,src2).itype.size,OperandContents(lvm_s0,src1),val.d);
+        assert OperandContents(lvm_s0,dst).Int?;
 
 
-    ghost var lvm_b2, lvm_s2 := lvm_lemma_Add(lvm_b1, lvm_s0, lvm_sM, src2, size,src1,val,o);
+    ghost var lvm_b2, lvm_s2 := lvm_lemma_Add(lvm_b1, lvm_s0, lvm_sM, src2, size,src1,val);
 
 
     assert OperandContents(lvm_s2, src2).val == step1.val;
     assert OperandContents(lvm_s2,src2).val == evalADD(size,OperandContents(lvm_s0,src1),OperandContents(lvm_s0,val)).val;
     assert OperandContents(lvm_s0, src1) == OperandContents(lvm_s2, src1); 
 
-    assert  lvm_require(lvm_b2, lvm_code_Add(dst, size,src2,val2), lvm_s2, lvm_sM,dst);
-    var step2 := evalADD(OperandContents(lvm_s2,dst).itype.size,OperandContents(lvm_s2,src2),val2.d);
+    assert  lvm_require(lvm_b2, lvm_code_Add(dst, size,src2,val2), lvm_s2, lvm_sM);
+    // assert ValidOperand(lvm_s2,dst);
+    // assert OperandContents(lvm_s2,dst).Int?;
+    // var step2 := evalADD(OperandContents(lvm_s2,dst).itype.size,OperandContents(lvm_s2,src2),val2.d);
 
-    ghost var lvm_b3, lvm_s3 := lvm_lemma_Add(lvm_b2, lvm_s2, lvm_sM, dst, size,src2,val2,o);
+    ghost var lvm_b3, lvm_s3 := lvm_lemma_Add(lvm_b2, lvm_s2, lvm_sM, dst, size,src2,val2);
     assert OperandContents(lvm_s3, dst).val 
         == evalADD(OperandContents(lvm_s2,dst).itype.size,OperandContents(lvm_s2,src2),val2.d).val;
   
-    assert OperandContents(lvm_s3, dst).val  == step2.val;
+    // assert OperandContents(lvm_s3, dst).val  == step2.val;
 
     assert lvm_b3.hd.ins == RET(D(Void));
 
@@ -338,12 +335,13 @@ lemma lvm_lemma_Add_Multiple1(lvm_b0:lvm_codes, lvm_s0:lvm_state, lvm_sN:lvm_sta
     assert lvm_b4.CNil?;
 
     lvm_sM := lvm_lemma_empty(lvm_s4,lvm_sM);
-    assert OperandContents(lvm_sM, dst).val  == step2.val;
-
-    assert evalCode_lax(lvm_cM, lvm_s0, lvm_sM,dst);
+    // assert OperandContents(lvm_sM, dst).val  == step2.val;
+    assert  OperandContents(lvm_s4, dst).val 
+        == evalADD(OperandContents(lvm_s2,dst).itype.size,OperandContents(lvm_s2,src2),val2.d).val;
+    assert evalCode_lax(lvm_cM, lvm_s0, lvm_sM);
     assert OperandContents(lvm_s0, src1) == OperandContents(lvm_sM, src1); 
 
-    assert OperandContents(lvm_sM, dst).val == step2.val;
+    // assert OperandContents(lvm_sM, dst).val == step2.val;
     assert  OperandContents(lvm_sM, dst).val == evalADD(OperandContents(lvm_s0,dst).itype.size,OperandContents(lvm_s0,src2),val2.d).val;
     assert ValidState(lvm_sM);
 
